do not use working set in initialisation for fixed random oracle,   use 'dom m \ univ' directly

examples/list-ddh/RandOracle.ec
@@ -5,15 +5,18 @@
 *)
 require import Map.
 require import FSet.
+require import ISet.
+  import ISet.Finite.
 require import Real.
+require import Int.
 require import Distr.
 
 theory RandOracle.
 
   (* finite type of oracle inputs *)
   type from.
-  const univ_from : from set.
-  axiom univ_from_all_mem : forall (x : from), mem x univ_from.
+  axiom from_univ_finite : finite ISet.univ<:from>.
+  op univ_from = toFSet (univ<:from>).
 
   type to.
 
@@ -48,10 +51,8 @@ theory RandOracle.
       var xs : from set;
       var y : to;
       m = Map.empty;
-      xs = univ_from;
-      while (xs <> FSet.empty) {
-        x  = pick xs;
-        xs = rm x xs;
+      while (toFSet (dom m) <> univ_from) {
+        x  = pick (filter (lambda x, ! mem x (toFSet (dom m))) univ_from);
         y  = $dsample;
         m = m.[ x <- y ];
       }
@@ -62,15 +63,13 @@ theory RandOracle.
   }.
 
   lemma LRO_lossless_query:
-    mu dsample Fun.cpTrue = 1%r => islossless LRO.query.
-    (* FIXME: cpTrue unqualified should work *)
-  proof strict.             
+    mu dsample cpTrue = 1%r => islossless LRO.query.
+  proof strict.
   intros=> samp.
   fun.
     if.
-      wp; rnd. smt.
+      wp; rnd; skip; smt.
     skip; smt.
-    skip. smt.
   qed.
 
   lemma LRO_lossless_init:
@@ -82,21 +81,28 @@ theory RandOracle.
   lemma FRO_lossless_query:
     islossless FRO.query.
   proof strict.
-  fun. skip; smt.
+    fun. skip; smt.
   qed.
 
   lemma FRO_lossless_init:
     mu dsample Fun.cpTrue = 1%r => islossless FRO.init.
   proof strict.
-  intros=> dsamp.
-  fun.
-  while true (card xs).
-  intros=> z.
-  wp. rnd. smt.
-  wp. skip.
-  intros=> &hr H.
-  elim H => noEmpty card. smt.
-  wp. skip. progress. smt.
+    intros=> dsamp.
+    fun.
+    while true (card (univ_from) - card (toFSet (dom FRO.m))).
+    intros=> z.
+    wp; rnd; wp.
+    skip; progress.
+    admit. (* lambda is equal to cpTrue *)
+    wp; skip; progress.
+    cut H1: card univ_from <= card (toFSet (dom m)); first smt.
+    cut H2: toFSet (dom m) <= univ_from; first smt.
+    case (toFSet (dom m) = univ_from); first smt.
+    intros => Hneq.
+    cut H3: toFSet (dom m) < univ_from; first by smt.
+    cut H4: card (toFSet (dom m)) < card (univ_from).
+      admit. (* there are some facts about card missing *)
+    smt.
   qed.
 
   (** Switching between lazy and fixed random oracle *)
@@ -138,7 +144,7 @@ theory RandOracle.
     inline LRO.init FRO.init.
     admit. (* This should be provable using eager if we add the same while loop
               to the end of the left game.
-              Note that U.f is abstract and only allowed to perform oracle queries.
+              Note that U.main is abstract and only allowed to perform oracle queries.
            *)
   qed.
 end RandOracle.
